Veir/Rewriter/GetSetInBounds.lean
@@ -2652,6 +2652,168 @@ theorem OpOperandPtrPtr.get!_initOpResults {opOperandPtr : OpOperandPtrPtr} :
 
 end Rewriter.initOpResults
 
+/-! ## `Rewriter.pushRegion` -/
+
+section Rewriter.pushRegion
+
+variable {op : OperationPtr}
+
+attribute [local grind] Rewriter.pushRegion
+
+@[simp, grind =]
+theorem BlockPtr.get!_pushRegion {block : BlockPtr} :
+    block.get! (Rewriter.pushRegion ctx op region hop hregion hregionParent) =
+    block.get! ctx := by
+  grind
+
+@[simp, grind =]
+theorem OperationPtr.prev!_pushRegion {operation : OperationPtr} :
+    (operation.get! (Rewriter.pushRegion ctx op region hop hregion hregionParent)).prev =
+    (operation.get! ctx).prev := by
+  grind
+
+@[simp, grind =]
+theorem OperationPtr.next!_pushRegion {operation : OperationPtr} :
+    (operation.get! (Rewriter.pushRegion ctx op region hop hregion hregionParent)).next =
+    (operation.get! ctx).next := by
+  grind
+
+@[simp, grind =]
+theorem OperationPtr.parent!_pushRegion {operation : OperationPtr} :
+    (operation.get! (Rewriter.pushRegion ctx op region hop hregion hregionParent)).parent =
+    (operation.get! ctx).parent := by
+  grind
+
+@[simp, grind =]
+theorem OperationPtr.opType!_pushRegion {operation : OperationPtr} :
+    (operation.get! (Rewriter.pushRegion ctx op region hop hregion hregionParent)).opType =
+    (operation.get! ctx).opType := by
+  grind
+
+@[simp, grind =]
+theorem OperationPtr.attrs!_pushRegion {operation : OperationPtr} :
+    (operation.get! (Rewriter.pushRegion ctx op region hop hregion hregionParent)).attrs =
+    (operation.get! ctx).attrs := by
+  grind
+
+@[simp, grind =]
+theorem OperationPtr.getProperties!_pushRegion {operation : OperationPtr} :
+    operation.getProperties! (Rewriter.pushRegion ctx op region hop hregion hregionParent) opCode =
+    operation.getProperties! ctx opCode := by
+  grind
+
+@[simp, grind =]
+theorem OperationPtr.getNumResults!_pushRegion {operation : OperationPtr} :
+    operation.getNumResults! (Rewriter.pushRegion ctx op region hop hregion hregionParent) =
+    operation.getNumResults! ctx := by
+  grind
+
+@[simp, grind =]
+theorem OpResultPtr.get!_pushRegion {opResult : OpResultPtr} :
+    opResult.get! (Rewriter.pushRegion ctx op region hop hregion hregionParent) =
+    opResult.get! ctx := by
+  grind
+
+@[simp, grind =]
+theorem OperationPtr.getNumOperands!_pushRegion {operation : OperationPtr} :
+    operation.getNumOperands! (Rewriter.pushRegion ctx op region hop hregion hregionParent) =
+    operation.getNumOperands! ctx := by
+  grind
+
+@[simp, grind =]
+theorem OpOperandPtr.get!_pushRegion {opOperand : OpOperandPtr} :
+    opOperand.get! (Rewriter.pushRegion ctx op region hop hregion hregionParent) =
+    opOperand.get! ctx := by
+  grind
+
+@[simp, grind =]
+theorem OperationPtr.getOperands!_pushRegion {operation : OperationPtr} :
+    operation.getOperands! (Rewriter.pushRegion ctx op region hop hregion hregionParent) =
+    operation.getOperands! ctx := by
+  grind
+
+@[simp, grind =]
+theorem OperationPtr.getNumSuccessors!_pushRegion {operation : OperationPtr} :
+    operation.getNumSuccessors! (Rewriter.pushRegion ctx op region hop hregion hregionParent) =
+    operation.getNumSuccessors! ctx := by
+  grind
+
+@[simp, grind =]
+theorem BlockOperandPtr.get!_pushRegion {blockOperand : BlockOperandPtr} :
+    blockOperand.get! (Rewriter.pushRegion ctx op region hop hregion hregionParent) =
+    blockOperand.get! ctx := by
+  grind
+
+@[grind =]
+theorem OperationPtr.getNumRegions!_pushRegion {operation : OperationPtr} :
+    operation.getNumRegions! (Rewriter.pushRegion ctx op region hop hregion hregionParent) =
+    if operation = op then operation.getNumRegions! ctx + 1
+    else operation.getNumRegions! ctx := by
+  grind
+
+@[grind =]
+theorem OperationPtr.getRegion!_pushRegion {operation : OperationPtr} :
+    operation.getRegion! (Rewriter.pushRegion ctx op region hop hregion hregionParent) index =
+    if operation = op ∧ index = operation.getNumRegions! ctx then region
+    else operation.getRegion! ctx index := by
+  grind
+
+@[simp, grind =]
+theorem BlockOperandPtrPtr.get!_pushRegion {blockOperandPtr : BlockOperandPtrPtr} :
+    blockOperandPtr.get! (Rewriter.pushRegion ctx op region hop hregion hregionParent) =
+    blockOperandPtr.get! ctx := by
+  grind
+
+@[simp, grind =]
+theorem BlockPtr.getNumArguments!_pushRegion {block : BlockPtr} :
+    block.getNumArguments! (Rewriter.pushRegion ctx op region hop hregion hregionParent) =
+    block.getNumArguments! ctx := by
+  grind
+
+@[simp, grind =]
+theorem BlockArgumentPtr.get!_pushRegion {blockArg : BlockArgumentPtr} :
+    blockArg.get! (Rewriter.pushRegion ctx op region hop hregion hregionParent) =
+    blockArg.get! ctx := by
+  grind
+
+@[simp, grind =]
+theorem RegionPtr.firstBlock!_pushRegion {r : RegionPtr} :
+    (r.get! (Rewriter.pushRegion ctx op region hop hregion hregionParent)).firstBlock =
+    (r.get! ctx).firstBlock := by
+  grind
+
+@[simp, grind =]
+theorem RegionPtr.lastBlock!_pushRegion {r : RegionPtr} :
+    (r.get! (Rewriter.pushRegion ctx op region hop hregion hregionParent)).lastBlock =
+    (r.get! ctx).lastBlock := by
+  grind
+
+@[grind =]
+theorem RegionPtr.parent!_pushRegion {r : RegionPtr} :
+    (r.get! (Rewriter.pushRegion ctx op region hop hregion hregionParent)).parent =
+    if r = region then some op else (r.get! ctx).parent := by
+  grind
+
+@[simp, grind =]
+theorem ValuePtr.getFirstUse!_pushRegion {value : ValuePtr} :
+    value.getFirstUse! (Rewriter.pushRegion ctx op region hop hregion hregionParent) =
+    value.getFirstUse! ctx := by
+  grind
+
+@[simp, grind =]
+theorem ValuePtr.getType!_pushRegion {value : ValuePtr} :
+    value.getType! (Rewriter.pushRegion ctx op region hop hregion hregionParent) =
+    value.getType! ctx := by
+  grind
+
+@[simp, grind =]
+theorem OpOperandPtrPtr.get!_pushRegion {opOperandPtr : OpOperandPtrPtr} :
+    opOperandPtr.get! (Rewriter.pushRegion ctx op region hop hregion hregionParent) =
+    opOperandPtr.get! ctx := by
+  grind
+
+end Rewriter.pushRegion
+
 /-! ## `Rewriter.initOpRegions` -/
 
 section Rewriter.initOpRegions
@@ -2660,157 +2822,164 @@ variable {op : OperationPtr}
 
 attribute [local grind] Rewriter.initOpRegions
 
-@[simp, grind =]
-theorem BlockPtr.get!_initOpRegions {block : BlockPtr} :
-    block.get! (Rewriter.initOpRegions ctx op regions index h₁ h₂ h₃ h₄) = block.get! ctx := by
+@[simp, grind =>]
+theorem BlockPtr.get!_initOpRegions {block : BlockPtr} {ctx' : IRContext OpInfo}
+    (h : Rewriter.initOpRegions ctx op regions index h₁ h₂ h₃ h₄ = some ctx') :
+    block.get! ctx' = block.get! ctx := by
   fun_induction Rewriter.initOpRegions <;> grind
 
-
-@[simp, grind =]
-theorem OperationPtr.prev!_initOpRegions {operation : OperationPtr} :
-    (operation.get! (Rewriter.initOpRegions ctx op regions index h₁ h₂ h₃ h₄)).prev =
-    (operation.get! ctx).prev := by
+@[simp, grind =>]
+theorem OperationPtr.prev!_initOpRegions {operation : OperationPtr} {ctx' : IRContext OpInfo}
+    (h : Rewriter.initOpRegions ctx op regions index h₁ h₂ h₃ h₄ = some ctx') :
+    (operation.get! ctx').prev = (operation.get! ctx).prev := by
   fun_induction Rewriter.initOpRegions <;> grind
 
-@[simp, grind =]
-theorem OperationPtr.next!_initOpRegions {operation : OperationPtr} :
-    (operation.get! (Rewriter.initOpRegions ctx op regions index h₁ h₂ h₃ h₄)).next =
-    (operation.get! ctx).next := by
+@[simp, grind =>]
+theorem OperationPtr.next!_initOpRegions {operation : OperationPtr} {ctx' : IRContext OpInfo}
+    (h : Rewriter.initOpRegions ctx op regions index h₁ h₂ h₃ h₄ = some ctx') :
+    (operation.get! ctx').next = (operation.get! ctx).next := by
   fun_induction Rewriter.initOpRegions <;> grind
 
-@[simp, grind =]
-theorem OperationPtr.parent!_initOpRegions {operation : OperationPtr} :
-    (operation.get! (Rewriter.initOpRegions ctx op regions index h₁ h₂ h₃ h₄)).parent =
-    (operation.get! ctx).parent := by
+@[simp, grind =>]
+theorem OperationPtr.parent!_initOpRegions {operation : OperationPtr} {ctx' : IRContext OpInfo}
+    (h : Rewriter.initOpRegions ctx op regions index h₁ h₂ h₃ h₄ = some ctx') :
+    (operation.get! ctx').parent = (operation.get! ctx).parent := by
   fun_induction Rewriter.initOpRegions <;> grind
 
-@[simp, grind =]
-theorem OperationPtr.opType!_initOpRegions {operation : OperationPtr} :
-    (operation.get! (Rewriter.initOpRegions ctx op regions index h₁ h₂ h₃ h₄)).opType =
-    (operation.get! ctx).opType := by
+@[simp, grind =>]
+theorem OperationPtr.opType!_initOpRegions {operation : OperationPtr} {ctx' : IRContext OpInfo}
+    (h : Rewriter.initOpRegions ctx op regions index h₁ h₂ h₃ h₄ = some ctx') :
+    (operation.get! ctx').opType = (operation.get! ctx).opType := by
   fun_induction Rewriter.initOpRegions <;> grind
 
-@[simp, grind =]
-theorem OperationPtr.attrs!_initOpRegions {operation : OperationPtr} :
-    (operation.get! (Rewriter.initOpRegions ctx op regions index h₁ h₂ h₃ h₄)).attrs =
-    (operation.get! ctx).attrs := by
+@[simp, grind =>]
+theorem OperationPtr.attrs!_initOpRegions {operation : OperationPtr} {ctx' : IRContext OpInfo}
+    (h : Rewriter.initOpRegions ctx op regions index h₁ h₂ h₃ h₄ = some ctx') :
+    (operation.get! ctx').attrs = (operation.get! ctx).attrs := by
   fun_induction Rewriter.initOpRegions <;> grind
 
-@[simp, grind =]
-theorem OperationPtr.getProperties!_initOpRegions {operation : OperationPtr} :
-    operation.getProperties! (Rewriter.initOpRegions ctx op regions index h₁ h₂ h₃ h₄) opCode =
-    operation.getProperties! ctx opCode := by
+@[simp, grind =>]
+theorem OperationPtr.getProperties!_initOpRegions {operation : OperationPtr} {ctx' : IRContext OpInfo}
+    (h : Rewriter.initOpRegions ctx op regions index h₁ h₂ h₃ h₄ = some ctx') :
+    operation.getProperties! ctx' opCode = operation.getProperties! ctx opCode := by
   fun_induction Rewriter.initOpRegions <;> grind
 
-@[simp, grind =]
-theorem OperationPtr.getNumOperands!_initOpRegions {operation : OperationPtr} :
-    operation.getNumOperands! (Rewriter.initOpRegions ctx op regions index h₁ h₂ h₃ h₄) =
-    operation.getNumOperands! ctx := by
+@[simp, grind =>]
+theorem OperationPtr.getNumOperands!_initOpRegions {operation : OperationPtr} {ctx' : IRContext OpInfo}
+    (h : Rewriter.initOpRegions ctx op regions index h₁ h₂ h₃ h₄ = some ctx') :
+    operation.getNumOperands! ctx' = operation.getNumOperands! ctx := by
   fun_induction Rewriter.initOpRegions <;> grind
 
-@[simp, grind =]
-theorem OpResultPtr.get!_initOpRegions {opResult : OpResultPtr} {index : Nat} {h₄} :
-    opResult.get! (Rewriter.initOpRegions ctx op regions index h₁ h₂ h₃ h₄) =
-    opResult.get! ctx := by
+@[simp, grind =>]
+theorem OpResultPtr.get!_initOpRegions {opResult : OpResultPtr}
+    (h : Rewriter.initOpRegions ctx op regions idx h₁ h₂ h₃ h₄ = some ctx') :
+    opResult.get! ctx' = opResult.get! ctx := by
   fun_induction Rewriter.initOpRegions <;> grind
 
-@[simp, grind =]
-theorem OpOperandPtr.get!_initOpRegions {opOperand : OpOperandPtr} {index} {h₄} :
-    opOperand.get! (Rewriter.initOpRegions ctx op regions index h₁ h₂ h₃ h₄) = opOperand.get! ctx := by
+@[simp, grind =>]
+theorem OpOperandPtr.get!_initOpRegions {opOperand : OpOperandPtr}
+    (h : Rewriter.initOpRegions ctx op regions idx h₁ h₂ h₃ h₄ = some ctx') :
+    opOperand.get! ctx' = opOperand.get! ctx := by
   fun_induction Rewriter.initOpRegions <;> grind
 
-@[simp, grind =]
-theorem OperationPtr.getOperands!_initOpRegions {operation : OperationPtr} {index} {h₄} :
-    operation.getOperands! (Rewriter.initOpRegions ctx op regions index h₁ h₂ h₃ h₄) = operation.getOperands! ctx := by
+@[simp, grind =>]
+theorem OperationPtr.getOperands!_initOpRegions {operation : OperationPtr}
+    (h : Rewriter.initOpRegions ctx op regions index h₁ h₂ h₃ h₄ = some ctx') :
+    operation.getOperands! ctx' = operation.getOperands! ctx := by
   fun_induction Rewriter.initOpRegions <;> grind
 
-@[simp, grind =]
-theorem OperationPtr.getNumSuccessors!_initOpRegions {operation : OperationPtr} :
-    operation.getNumSuccessors! (Rewriter.initOpRegions ctx op regions index h₁ h₂ h₃ h₄) =
-    operation.getNumSuccessors! ctx := by
+@[simp, grind =>]
+theorem OperationPtr.getNumSuccessors!_initOpRegions {operation : OperationPtr}
+    (h : Rewriter.initOpRegions ctx op regions index h₁ h₂ h₃ h₄ = some ctx') :
+    operation.getNumSuccessors! ctx' = operation.getNumSuccessors! ctx := by
   fun_induction Rewriter.initOpRegions <;> grind
 
-@[simp, grind =]
-theorem BlockOperandPtr.get!_initOpRegions {blockOperand : BlockOperandPtr} {index} {h₄} :
-    blockOperand.get! (Rewriter.initOpRegions ctx op regions index h₁ h₂ h₃ h₄) =
-    blockOperand.get! ctx := by
+@[simp, grind =>]
+theorem BlockOperandPtr.get!_initOpRegions {blockOperand : BlockOperandPtr}
+    (h : Rewriter.initOpRegions ctx op regions idx h₁ h₂ h₃ h₄ = some ctx') :
+    blockOperand.get! ctx' = blockOperand.get! ctx := by
   fun_induction Rewriter.initOpRegions <;> grind
 
-@[grind =]
-theorem OperationPtr.getNumRegions!_initOpRegions {operation : OperationPtr} :
-    operation.getNumRegions! (Rewriter.initOpRegions ctx op regions index h₁ h₂ h₃ h₄) =
+@[grind =>]
+theorem OperationPtr.getNumRegions!_initOpRegions {operation : OperationPtr}
+    (h : Rewriter.initOpRegions ctx op regions index h₁ h₂ h₃ h₄ = some ctx') :
+    operation.getNumRegions! ctx' =
     if operation = op then op.getNumRegions! ctx + (regions.size - index) else operation.getNumRegions! ctx := by
   fun_induction Rewriter.initOpRegions <;> grind
 
-@[simp, grind =]
-theorem OperationPtr.getRegion!_initOpRegions {operation : OperationPtr} :
-    operation.getRegion! (Rewriter.initOpRegions ctx op regions index h₁ h₂ h₃ h₄) idx =
+@[simp, grind =>]
+theorem OperationPtr.getRegion!_initOpRegions {operation : OperationPtr}
+    (h : Rewriter.initOpRegions ctx op regions index h₁ h₂ h₃ h₄ = some ctx') :
+    operation.getRegion! ctx' idx =
     if _ : operation = op ∧ idx ≥ op.getNumRegions! ctx ∧ idx < regions.size then regions[idx]
     else operation.getRegion! ctx idx := by
   fun_induction Rewriter.initOpRegions <;> grind (splits := 15)
 
-@[simp, grind =]
-theorem BlockOperandPtrPtr.get!_initOpRegions {blockOperandPtr : BlockOperandPtrPtr} :
-    blockOperandPtr.get! (Rewriter.initOpRegions ctx op regions index h₁ h₂ h₃ h₄) =
-    blockOperandPtr.get! ctx := by
+@[simp, grind =>]
+theorem BlockOperandPtrPtr.get!_initOpRegions {blockOperandPtr : BlockOperandPtrPtr}
+    (h : Rewriter.initOpRegions ctx op regions index h₁ h₂ h₃ h₄ = some ctx') :
+    blockOperandPtr.get! ctx' = blockOperandPtr.get! ctx := by
   fun_induction Rewriter.initOpRegions <;> grind
 
-@[simp, grind =]
-theorem BlockPtr.getNumArguments!_initOpRegions {block : BlockPtr} :
-    block.getNumArguments! (Rewriter.initOpRegions ctx op regions index h₁ h₂ h₃ h₄) =
-    block.getNumArguments! ctx := by
+@[simp, grind =>]
+theorem BlockPtr.getNumArguments!_initOpRegions {block : BlockPtr}
+    (h : Rewriter.initOpRegions ctx op regions index h₁ h₂ h₃ h₄ = some ctx') :
+    block.getNumArguments! ctx' = block.getNumArguments! ctx := by
   fun_induction Rewriter.initOpRegions <;> grind
 
-@[simp, grind =]
-theorem BlockArgumentPtr.get!_initOpRegions {blockArg : BlockArgumentPtr} {index} {h₄} :
-    blockArg.get! (Rewriter.initOpRegions ctx op regions index h₁ h₂ h₃ h₄) =
-    blockArg.get! ctx := by
+@[simp, grind =>]
+theorem BlockArgumentPtr.get!_initOpRegions {blockArg : BlockArgumentPtr}
+    (h : Rewriter.initOpRegions ctx op regions idx h₁ h₂ h₃ h₄ = some ctx') :
+    blockArg.get! ctx' = blockArg.get! ctx := by
   fun_induction Rewriter.initOpRegions <;> grind
 
-@[simp, grind =]
-theorem RegionPtr.firstBlock!_initOpRegions {region : RegionPtr} :
-    (region.get! (Rewriter.initOpRegions ctx op regions index h₁ h₂ h₃ h₄)).firstBlock =
-    (region.get! ctx).firstBlock := by
+@[simp, grind =>]
+theorem RegionPtr.firstBlock!_initOpRegions {region : RegionPtr}
+    (h : Rewriter.initOpRegions ctx op regions index h₁ h₂ h₃ h₄ = some ctx') :
+    (region.get! ctx').firstBlock = (region.get! ctx).firstBlock := by
   fun_induction Rewriter.initOpRegions <;> grind (instances := 5000)
 
-@[simp, grind =]
-theorem RegionPtr.lastBlock!_initOpRegions {region : RegionPtr} :
-    (region.get! (Rewriter.initOpRegions ctx op regions index h₁ h₂ h₃ h₄)).lastBlock =
-    (region.get! ctx).lastBlock := by
+@[simp, grind =>]
+theorem RegionPtr.lastBlock!_initOpRegions {region : RegionPtr}
+    (h : Rewriter.initOpRegions ctx op regions index h₁ h₂ h₃ h₄ = some ctx') :
+    (region.get! ctx').lastBlock = (region.get! ctx).lastBlock := by
   fun_induction Rewriter.initOpRegions <;> grind (instances := 5000)
 
-theorem RegionPtr.parent!_initOpRegions_gen {region : RegionPtr} :
-    (region.get! (Rewriter.initOpRegions ctx op regions index h₁ h₂ h₃ h₄)).parent =
+theorem RegionPtr.parent!_initOpRegions_gen {region : RegionPtr}
+    (h : Rewriter.initOpRegions ctx op regions index h₁ h₂ h₃ h₄ = some ctx') :
+    (region.get! ctx').parent =
     if ∃ (i : Nat) (_ : i < regions.size), index ≤ i ∧ regions[i] = region then some op else (region.get! ctx).parent := by
   fun_induction Rewriter.initOpRegions
   · grind (instances := 5000) (gen := 100)
   · simp_all +zetaDelta only
     split <;> split <;> grind (instances := 5000)
+  · grind
 
-@[grind =]
-theorem RegionPtr.parent!_initOpRegions {region : RegionPtr} :
-    (region.get! (Rewriter.initOpRegions ctx op regions 0 h₁ h₂ h₃ h₄)).parent =
+@[grind =>]
+theorem RegionPtr.parent!_initOpRegions {region : RegionPtr}
+    (h : Rewriter.initOpRegions ctx op regions 0 h₁ h₂ h₃ h₄ = some ctx') :
+    (region.get! ctx').parent =
     if region ∈ regions then some op else (region.get! ctx).parent := by
-  rw [parent!_initOpRegions_gen]
+  rw [parent!_initOpRegions_gen h]
   congr
   grind [Array.mem_iff_getElem]
 
-@[simp, grind =]
-theorem ValuePtr.getFirstUse!_initOpRegions {value : ValuePtr} :
-    value.getFirstUse! (Rewriter.initOpRegions ctx op regions index h₁ h₂ h₃ h₄) =
-    value.getFirstUse! ctx := by
+@[simp, grind =>]
+theorem ValuePtr.getFirstUse!_initOpRegions {value : ValuePtr}
+    (h : Rewriter.initOpRegions ctx op regions index h₁ h₂ h₃ h₄ = some ctx') :
+    value.getFirstUse! ctx' = value.getFirstUse! ctx := by
   fun_induction Rewriter.initOpRegions <;> grind
 
-@[simp, grind =]
-theorem ValuePtr.getType!_initOpRegions {value : ValuePtr} :
-    value.getType! (Rewriter.initOpRegions ctx op regions index h₁ h₂ h₃ h₄) =
-    value.getType! ctx := by
+@[simp, grind =>]
+theorem ValuePtr.getType!_initOpRegions {value : ValuePtr}
+    (h : Rewriter.initOpRegions ctx op regions index h₁ h₂ h₃ h₄ = some ctx') :
+    value.getType! ctx' = value.getType! ctx := by
   fun_induction Rewriter.initOpRegions <;> grind
 
-@[simp, grind =]
-theorem OpOperandPtrPtr.get!_initOpRegions {opOperandPtr : OpOperandPtrPtr} :
-    opOperandPtr.get! (Rewriter.initOpRegions ctx op regions index h₁ h₂ h₃ h₄) =
-    opOperandPtr.get! ctx := by
+@[simp, grind =>]
+theorem OpOperandPtrPtr.get!_initOpRegions {opOperandPtr : OpOperandPtrPtr}
+    (h : Rewriter.initOpRegions ctx op regions index h₁ h₂ h₃ h₄ = some ctx') :
+    opOperandPtr.get! ctx' = opOperandPtr.get! ctx := by
   fun_induction Rewriter.initOpRegions <;> grind
 
 end Rewriter.initOpRegions
@@ -4056,25 +4225,22 @@ theorem Rewriter.createOp_inBounds_mono (ptr : GenericPtr)
   simp only [createOp] at heq
   split at heq; grind
   split at heq
-  · split at heq; grind
-    intros hptr
-    rename_i h
-    simp at heq
-    have ⟨_, _⟩ := heq
-    subst newOp
-    subst newCtx
-    rw [←Rewriter.insertOp?_inBounds_mono ptr h]
-    grind
-  · grind (ematch := 10)
+  · grind
+  · split at heq
+    · split at heq; grind
+      intros hptr
+      rename_i h
+      simp at heq
+      have ⟨_, _⟩ := heq
+      subst newOp
+      subst newCtx
+      rw [←Rewriter.insertOp?_inBounds_mono ptr h]
+      grind
+    · grind
 
 @[grind .]
 theorem Rewriter.createOp_fieldsInBounds
     (heq : createOp ctx opType numResults operands blockOperands numRegions props ip h₁ h₂ h₃ h₄ h₅ = some (newCtx, newOp)) :
     ctx.FieldsInBounds → newCtx.FieldsInBounds := by
   simp only [createOp] at heq
-  split at heq; grind
-  split at heq
-  · split at heq
-    · grind
-    · grind
-  · grind
+  grind
