Veir/Rewriter/WellFormed/Builder/OpRegion.lean
@@ -1,15 +1,84 @@
 import Veir.IR.Basic
 import Veir.IR.WellFormed
-import Veir.Rewriter.Basic
+import Veir.Rewriter.GetSetInBounds
 
 namespace Veir
 
 variable {OpInfo : Type} [HasOpInfo OpInfo]
 variable {ctx : IRContext OpInfo}
 
-set_option warn.sorry false in
+theorem IRContext.wellFormed_Rewriter_pushRegion :
+    ctx.WellFormed →
+    (Rewriter.pushRegion ctx op region hop hregion hregionParent).WellFormed := by
+  intro wf
+  constructor
+  case valueDefUseChains =>
+    intros valuePtr valuePtrInBounds
+    have ⟨array, arrayWf⟩ := wf.valueDefUseChains valuePtr (by grind)
+    exists array
+    apply ValuePtr.DefUse.unchanged (ctx := ctx) <;> grind
+  case blockDefUseChains =>
+    intros blockPtr blockPtrInBounds
+    have ⟨array, arrayWf⟩ := wf.blockDefUseChains blockPtr (by grind)
+    exists array
+    apply BlockPtr.DefUse.unchanged (ctx := ctx) <;> grind
+  case inBounds => grind
+  case opChain =>
+    intros blockPtr blockPtrInBounds
+    have ⟨array, arrayWf⟩ := wf.opChain blockPtr (by grind)
+    exists array
+    apply BlockPtr.OpChain_unchanged (ctx := ctx) <;>
+      grind
+  case blockChain =>
+    intros reg hreg
+    have ⟨array, arrayWf⟩ := wf.blockChain reg (by grind)
+    exists array
+    apply RegionPtr.blockChain_unchanged (ctx := ctx) <;>
+      grind
+  case operations =>
+    intros opPtr' opPtrInBounds
+    have ⟨h₁, h₂, h₃, h₄, h₅, h₆, h₇, h₈⟩ := wf.operations opPtr' (by grind)
+    constructor
+    case region_parent =>
+      intros region' region'InBounds
+      constructor
+      · grind
+      · simp only [RegionPtr.parent!_pushRegion]
+        split; rotate_left; grind
+        intro _
+        exists op.getNumRegions! ctx
+        grind
+    all_goals grind [Operation.WellFormed]
+  case blocks =>
+    intros bl hbl
+    constructor
+    · grind
+    · intros i hi
+      have ⟨h₁, h₂, h₃⟩ := wf.blocks bl (by grind)
+      grind
+    · intros i hi
+      have ⟨h₁, h₂, h₃⟩ := wf.blocks bl (by grind)
+      grind
+  case regions =>
+    intros reg hreg
+    have ⟨h₁, h₂⟩ := wf.regions reg (by grind)
+    constructor
+    · grind [Rewriter.pushOperand]
+    · simp only [RegionPtr.parent!_pushRegion]
+      split
+      · simp only [Option.some.injEq, forall_eq']
+        exists op.getNumRegions! ctx
+        grind
+      · intro parent hparent
+        have ⟨i, hi⟩ := h₂ hparent
+        grind
+
 theorem Rewriter.initOpRegions_WellFormed (opPtr: OperationPtr)
-    (hop : opPtr.InBounds ctx) (hctx : IRContext.WellFormed ctx) {hn} (newCtx : IRContext OpInfo):
-    Rewriter.initOpRegions ctx opPtr regions n hop regionInBounds (by grind) hn = some newCtx →
-    newCtx.WellFormed := by
-  sorry
+    (hop : opPtr.InBounds ctx) (hfields : ctx.FieldsInBounds) (hctx : IRContext.WellFormed ctx) {hn}
+    {ctx' : IRContext OpInfo}
+    (h : Rewriter.initOpRegions ctx opPtr regions n hop regionInBounds hfields hn = some ctx') :
+    ctx'.WellFormed := by
+  fun_induction Rewriter.initOpRegions
+  case case1 => grind
+  case case2 => grind [IRContext.wellFormed_Rewriter_pushRegion]
+  case case3 => grind
